simrel_cert_graph_start lemma --- done

Coq/src/SimRelStep.v
@@ -1,5 +1,6 @@
 Require Import Omega.
 From hahn Require Import Hahn.
+From promising Require Import Basic.
 From imm Require Import Events Execution
      Traversal TraversalConfig SimTraversal SimTraversalProperties
      Prog ProgToExecution ProgToExecutionProperties Receptiveness
@@ -141,6 +142,97 @@ Section SimRelStep.
   Notation "'ktid' S" := (fun k => ES.cont_thread S k) (at level 1, only parsing).
 
   Notation "'certX' S" := (fun k => (X ∩₁ SNTid_ S (ktid S k)) ∪₁ (kE S k)) (at level 1, only parsing).
+
+  Definition cont_pc S X k thread := 
+    (<< KREP : k = CInit thread >> /\
+     << CEMP : C ∩₁ GTid thread ≡₁ ∅ >>) 
+    \/
+    (exists e,
+        << KREP : k = CEvent e >> /\
+        << Xe   : X e >> /\
+        << EPC  : pc G TC thread (e2a S e) >> 
+    ).
+
+  Lemma simrel_cert_cont_pc S thread 
+        (NINITT : thread <> tid_init)
+        (SRC : simrel prog S G sc TC X) 
+        (TC_STEP : isim_trav_step G sc thread TC TC') : 
+    exists k (state : Language.state (thread_lts thread)),
+      ⟪ THK : thread = ES.cont_thread S k ⟫ /\
+      ⟪ INK : K S (k, thread_cont_st thread state) ⟫ /\
+      ⟪ EST : state.(ProgToExecution.G).(acts_set) ≡₁
+                  C ∩₁ GTid thread ⟫ /\
+      ⟪ kPC : cont_pc S X k thread ⟫.
+  Proof. 
+    cdes SRC.
+    assert (ES.Wf S) as WFS by apply SRC.
+    assert (Wf G) as WF by apply SRC.
+    assert (simrel_graph G TC) as SG by apply SRC.
+    pose proof TC_STEP as HH. 
+    eapply trstep_thread_prog in HH; try apply SRC.
+    apply Basic.IdentMap.Facts.in_find_iff in HH.
+    destruct (Basic.IdentMap.find thread (stable_prog_to_prog prog))
+      as [lprog|] eqn:AA; desf.
+    destruct (classic (exists x, (C ∩₁ GTid thread) x)) as [[x [CX TX]]|NN].
+    2: { exists (CInit thread).
+         edestruct contrun as [st]; try apply SRC; eauto. 
+         desf.
+         eexists. splits; eauto.
+         2: { left. eexists. splits; eauto.
+              generalize NN. basic_solver. }
+         etransitivity.
+         { eapply steps_empty_same_E; eauto. }
+         arewrite (C ∩₁ GTid thread ≡₁ ∅).
+         { generalize NN. basic_solver. }
+         simpls. }
+    edestruct exists_pc as [xpc XPC]; eauto; try apply SRC.
+    assert ((e2a S □₁ X) xpc) as EE.
+    { eapply ex_cov_iss; eauto. left. apply XPC. }
+    red in EE. desf.
+    assert (Gtid x = Stid S y) as TT.
+    { rewrite e2a_tid. red in XPC. generalize XPC. basic_solver. }
+    rewrite TT in XPC.
+    edestruct ES.event_K with (e:=y) as [c INKC]; try apply SRC.
+    { split.
+      { eapply Execution.ex_inE; eauto. apply SRC. }
+      intros [CC BB].
+      rewrite <- TT in BB. desf. }
+    { intros [z RMW].
+      apply XPC. exists (e2a S z).
+      assert (Grmw (e2a S y) (e2a S z)) as GRMW.
+      { eapply e2a_rmw; try apply SRC.
+        red. eauto. }
+      apply seq_eqv_r. split.
+      { apply rmw_in_sb; auto. }
+      erewrite <- rmwclos. 
+      { apply XPC. }
+      all: eauto. }
+    destruct c as [lang state].
+    set (BB := INKC).
+    eapply contlang in BB; try apply SRC.
+    desf.
+    exists (CEvent y). exists state.
+    splits; eauto.
+    { arewrite (Gtid x = ES.cont_thread S (CEvent y)). eauto. }
+    2: { right. eexists. split; eauto. by rewrite TT. }
+    (* TODO: generalize to a lemma *)
+    set (WFTS:=INKC).
+    eapply contwf in WFTS; try apply SRC.
+    simpls. rewrite <- TT in WFTS.
+    set (SS:=INKC).
+    eapply contpc in SS; try apply SRC; auto.
+    split.
+    { intros e CC.
+      set (DD:=CC).
+      eapply acts_rep in DD; eauto. desf.
+      split; auto.
+      cdes SS. rewrite TT. by apply PCOV. }
+    intros e [CC ET].
+    destruct e; simpls; desf.
+    { by rewrite ET in NINITT. }
+    cdes SS. rewrite TT in CC. apply PCOV in CC.
+    apply acts_clos; auto. 
+  Qed.
   
   Lemma simrel_cert_graph_start thread S 
         (NINITT : thread <> tid_init)
@@ -148,94 +240,25 @@ Section SimRelStep.
         (TC_STEP : isim_trav_step G sc thread TC TC') : 
     exists k st st',
       ⟪ kTID : thread = ktid S k ⟫ /\
-      ⟪ XkTIDCOV : kE S k ≡₁ X ∩₁ Stid_ S (ktid S k) ∩₁ e2a S ⋄₁ C ⟫ /\
+      ⟪ XkTIDCOV : kE S k ≡₁ X ∩₁ e2a S ⋄₁ C ∩₁ (SEinit S ∪₁ Stid_ S (ktid S k)) ⟫ /\
       ⟪ CERTG : cert_graph G sc TC TC' thread st' ⟫ /\
       ⟪ CERT_ST : simrel_cstate S k st st' ⟫.
   Proof.
     cdes SRC.
     assert (ES.Wf S) as WFS by apply SRC.
     assert (Wf G) as WF by apply SRC.
+    assert (Execution.t S X) as EXEC by apply SRC.
+    assert (simrel_e2a S G sc) as SRE2A by apply SRC.
 
-    pose proof TC_STEP as HH. 
+    pose proof TC_STEP as HH.
     eapply trstep_thread_prog in HH; try apply SRC.
     apply Basic.IdentMap.Facts.in_find_iff in HH.
     destruct (Basic.IdentMap.find thread (stable_prog_to_prog prog))
       as [lprog|] eqn:AA; desf.
-    
-    (* TODO: make it a separate lemma. *)
-    assert
-      (exists k (state : Language.state (thread_lts thread)),
-          ⟪ INK : K S (k, thread_cont_st thread state) ⟫ /\
-          ⟪ THK : thread = ES.cont_thread S k ⟫ /\
-          ⟪ EST : state.(ProgToExecution.G).(acts_set) ≡₁
-                  C ∩₁ GTid thread ⟫ /\
-          ((exists thread,
-               << KREP : k = CInit thread >> /\
-               << CEMP : C ∩₁ GTid thread ≡₁ ∅ >>) \/
-           (exists e,
-               << KREP : k = CEvent e >> /\
-               << EPC  : pc G TC thread (e2a S e) >>))
-      ).
-    { destruct (classic (exists x, (C ∩₁ GTid thread) x)) as [[x [CX TX]]|NN].
-      2: { exists (CInit thread).
-           edestruct contrun as [st]; try apply SRC; eauto. 
-           desf.
-           eexists. splits; eauto.
-           2: { left. eexists. splits; eauto.
-                generalize NN. basic_solver. }
-           etransitivity.
-           { eapply steps_empty_same_E; eauto. }
-           arewrite (C ∩₁ GTid thread ≡₁ ∅).
-           { generalize NN. basic_solver. }
-           simpls. }
-      edestruct exists_pc as [xpc XPC]; eauto; try apply SRC.
-      assert ((e2a S □₁ X) xpc) as EE.
-      { eapply ex_cov_iss; eauto. left. apply XPC. }
-      red in EE. desf.
-      assert (Gtid x = Stid S y) as TT.
-      { rewrite e2a_tid. red in XPC. generalize XPC. basic_solver. }
-      rewrite TT in XPC.
-      edestruct ES.event_K with (e:=y) as [c INKC]; try apply SRC.
-      { split.
-        { eapply Execution.ex_inE; eauto. apply SRC. }
-        intros [CC BB].
-        rewrite <- TT in BB. desf. }
-      { intros [z RMW].
-        apply XPC. exists (e2a S z).
-        assert (Grmw (e2a S y) (e2a S z)) as GRMW.
-        { eapply e2a_rmw; try apply SRC.
-          red. eauto. }
-        apply seq_eqv_r. split.
-        { apply rmw_in_sb; auto. }
-        eapply (rmwclos _ _ _ GRMW).
-          by apply XPC. }
-      destruct c as [lang state].
-      set (BB := INKC).
-      eapply contlang in BB; try apply SRC.
-      desf.
-      exists (CEvent y). exists state.
-      splits; eauto.
-      { arewrite (Gtid x = ES.cont_thread S (CEvent y)). eauto. }
-      2: { right. eexists. split; eauto. by rewrite TT. }
-      (* TODO: generalize to a lemma *)
-      set (WFTS:=INKC).
-      eapply contwf in WFTS; try apply SRC.
-      simpls. rewrite <- TT in WFTS.
-      set (SS:=INKC).
-      eapply contpc in SS; try apply SRC; auto.
-      split.
-      { intros e CC.
-        set (DD:=CC).
-        eapply acts_rep in DD; eauto. desf.
-        split; auto.
-        cdes SS. rewrite TT. by apply PCOV. }
-      intros e [CC ET].
-      destruct e; simpls; desf.
-      { by rewrite ET in NINITT. }
-      cdes SS. rewrite TT in CC. apply PCOV in CC.
-      apply acts_clos; auto. }
 
-    desc.
+    pose proof simrel_cert_cont_pc as CONTPC.
+    specialize (CONTPC S thread NINITT SRC TC_STEP).
+    desc. unfold cont_pc in kPC.
     assert (lprog = instrs state) as UU.
     { rewrite THK in *. eapply kstate_instrs; eauto; try apply SRC. }
 
@@ -252,6 +275,7 @@ Section SimRelStep.
       eapply contreach; eauto. apply SRC. }
     { desf.
       2: { eapply contpc; eauto. apply SRC. }
+      rewrite KREP in INK.
       eapply continitstate; simpls; eauto; try apply SRC.
       simpls. apply CEMP. }
     { rewrite EST. basic_solver. }
@@ -268,11 +292,81 @@ Section SimRelStep.
          { eapply contstable; try apply SRC; eauto.
            rewrite <- THK. eauto. }
          apply seq_eqv_r. by split. }
-    desf; simpls.
-    { (* TODO: it's wrong! *) admit. }
-    (* TODO: it's wrong! *)
-    admit.
-  Admitted.
+
+    split. 
+    { rewrite !set_subset_inter_r; splits.
+      { unfold ES.cont_sb_dom. 
+        desf; simpls. 
+        { eapply Execution.init_in_ex; eauto. }
+        arewrite (eq e ⊆₁ X).
+        { basic_solver. }
+        rewrite crE. 
+        relsf; splits; auto.
+        by apply Execution.ex_sb_prcl. }
+      { unfold ES.cont_sb_dom. 
+        desf; simpls. 
+        { eapply init_in_map_cov; eauto. }
+        arewrite (eq e ⊆₁ e2a S ⋄₁ C).
+        { unfolder. ins. desf. apply EPC. }
+        rewrite crE. 
+        relsf; splits; auto.
+        eapply sb_cov; eauto. }
+      eapply ES.cont_sb_tid; eauto. }
+    rewrite set_inter_union_r. unionL.
+    { apply set_subset_inter_l. right.
+      eapply ES.cont_sb_dom_Einit; eauto. }
+    unfold ES.cont_sb_dom. 
+    desf; simpls. 
+    { unfolder. ins. desf.
+      exfalso. eapply CEMP.
+      split; eauto.
+      by erewrite e2a_tid. }
+    rewrite crE. relsf.
+    unfolder. ins. desf. 
+    assert (~ cf S x e) as nCF.
+    { intros CF. 
+      eapply Execution.ex_ncf; eauto.
+      basic_solver. }
+    assert (SEninit S e) as nINITe.
+    { eapply ES.K_inEninit; eauto. }
+    edestruct ES.same_thread_alt as [SB | CF]; 
+      eauto; try done.
+    { eapply Execution.ex_inE; eauto. }
+    unfolder in SB. desf; eauto.
+    exfalso. 
+    assert (Gsb (e2a S x) (e2a S e)) as GSB.
+    { edestruct tid_sb as [GSB | [INITx INITe]].
+      { apply seq_eqv_lr. splits.
+        { eapply e2a_GE; eauto.
+          unfolder. eexists. splits; eauto.
+          eapply Execution.ex_inE; eauto. }
+        { red. rewrite <- !e2a_tid; eauto. }
+        eapply e2a_GE; eauto.
+        unfolder. eexists. splits; eauto.
+        eapply Execution.ex_inE; eauto. }
+      { unfolder in GSB. desf; auto.
+        { exfalso. eapply ES.sb_irr; eauto.
+          assert (e = x) as EQ.
+          { eapply e2a_inj with (X := X); eauto.
+            { eapply Execution.ex_inE; eauto. }
+            eapply Execution.ex_ncf; eauto. }
+          subst x. eauto. }
+        exfalso. 
+        apply EPC.
+        basic_solver 10. }
+      exfalso. 
+      eapply e2a_Eninit; eauto.
+      { apply SRE2A. }
+      basic_solver. }
+    eapply sb_irr. 
+    eapply sb_trans; eauto.
+    eapply e2a_sb; try apply SRC. 
+    (* TODO: make a lemma *)
+    { intros PROG_INIT. apply SRC_.(noinitprog).
+      unfold stable_prog_to_prog in PROG_INIT.
+      eapply IdentMap.map_2; eauto. }
+    basic_solver 10. 
+  Qed.
   
   Lemma simrel_cert_start k S 
         (st st' : thread_st (ktid S k))
